build.sh
@@ -6,5 +6,5 @@ makeit Metatheory_Var Metatheory_Fresh Metatheory_Env
 makeit Metatheory_SP Metatheory
 makeit ML_SP_Definitions ML_SP_Infrastructure
 makeit ML_SP_Soundness ML_SP_Rename ML_SP_Eval
-makeit Cardinal ML_SP_Unify ML_SP_Inference
+makeit Cardinal ML_SP_Unify_wf ML_SP_Inference_wf
 makeit ML_SP_Domain
